veric/env_pred.v
@@ -1,0 +1,209 @@
+Set Warnings "-notation-overridden,-custom-entry-overridden,-hiding-delimiting-key".
+Require Import VST.veric.res_predicates.
+Set Warnings "notation-overridden,custom-entry-overridden,hiding-delimiting-key".
+Require Import VST.veric.mpred.
+Require Import VST.veric.seplog.
+Require Import VST.veric.tycontext.
+Require Import VST.veric.Cop2.
+
+(* VeriC's assertions are functions environ -> mpred. *)
+
+Definition env_index : biIndex := {| bi_index_type := environ; bi_index_rel := eq |}.
+
+Definition assert `{!heapGS Σ} := monPred env_index (iPropI Σ).
+
+Program Definition assert_of `{!heapGS Σ} (P : environ -> mpred) : assert := {| monPred_at := P |}.
+
+Section assert.
+
+Context `{!heapGS Σ}.
+
+Record ret_assert : Type := {
+ RA_normal: assert;
+ RA_break: assert;
+ RA_continue: assert;
+ RA_return: option val -> assert
+}.
+
+Global Instance ret_assert_equiv : Equiv (ret_assert) := fun a b =>
+  (RA_normal a ⊣⊢ RA_normal b) /\ (RA_break a ⊣⊢ RA_break b) /\
+  (RA_continue a ⊣⊢ RA_continue b) /\ (forall v, RA_return a v ⊣⊢ RA_return b v).
+
+Global Instance ret_assert_equivalence : Equivalence (@base.equiv ret_assert _).
+Proof.
+  split.
+  - intros ?; hnf; auto.
+  - intros ?? (? & ? & ? & ?); split3; last split; intros; auto.
+    rewrite -H2 //.
+  - intros ??? (? & ? & ? & ?) (? & ? & ? & ?); split3; last split; intros; etrans; eauto.
+Qed.
+
+Definition proj_ret_assert (Q: ret_assert) (ek: exitkind) (vl: option val) : assert :=
+ match ek with
+ | EK_normal => ⌜vl=None⌝ ∧ RA_normal Q
+ | EK_break => ⌜vl=None⌝ ∧ RA_break Q
+ | EK_continue => ⌜vl=None⌝ ∧ RA_continue Q
+ | EK_return => RA_return Q vl
+ end.
+
+Definition overridePost  (Q: assert)  (R: ret_assert) :=
+  {| RA_normal := Q; RA_break := RA_break R; RA_continue := RA_continue R; RA_return := RA_return R |}.
+
+Definition existential_ret_assert {A: Type} (R: A -> ret_assert) :=
+  {| RA_normal := ∃ x:A, (R x).(RA_normal);
+     RA_break := ∃ x:A, (R x).(RA_break);
+     RA_continue := ∃ x:A, (R x).(RA_continue);
+     RA_return := fun vl => ∃ x:A, (R x).(RA_return) vl
+   |}.
+
+Definition normal_ret_assert (Q: assert) : ret_assert :=
+  {| RA_normal := Q; RA_break := False; RA_continue := False; RA_return := fun _ => False |}.
+
+Definition frame_ret_assert (R: ret_assert) (F: assert) : ret_assert :=
+  {| RA_normal := RA_normal R ∗ F;
+     RA_break := RA_break R ∗ F;
+     RA_continue := RA_continue R ∗ F;
+     RA_return := fun vl => RA_return R vl ∗ F |}.
+
+Definition conj_ret_assert (R: ret_assert) (F: assert) : ret_assert :=
+  {| RA_normal := RA_normal R ∧ F;
+     RA_break := RA_break R ∧ F;
+     RA_continue := RA_continue R ∧ F;
+     RA_return := fun vl => RA_return R vl ∧ F |}.
+
+Definition switch_ret_assert (R: ret_assert) : ret_assert :=
+  {| RA_normal := False; 
+     RA_break := RA_normal R;
+     RA_continue := RA_continue R;
+     RA_return := RA_return R |}.
+
+Lemma normal_ret_assert_derives:
+ forall P Q,
+  (P ⊢ Q) ->
+  forall ek vl, proj_ret_assert (normal_ret_assert P) ek vl
+            ⊢ proj_ret_assert (normal_ret_assert Q) ek vl.
+Proof.
+  intros.
+  destruct ek; simpl; auto.
+  rewrite H //.
+Qed.
+
+Lemma normal_ret_assert_False:
+  forall ek vl, proj_ret_assert (normal_ret_assert False) ek vl ⊣⊢ False.
+Proof.
+intros.
+destruct ek; simpl; auto; by rewrite bi.and_False.
+Qed.
+
+Lemma frame_normal:
+  forall P F, base.equiv (frame_ret_assert (normal_ret_assert P) F) (normal_ret_assert (P ∗ F)).
+Proof.
+intros.
+unfold normal_ret_assert; simpl.
+split3; last split; simpl; auto; intros; rewrite bi.sep_False //.
+Qed.
+
+Lemma pure_and_sep_assoc: forall {PROP} P (Q R : bi_car PROP), ⌜P⌝ ∧ Q ∗ R ⊣⊢ (⌜P⌝ ∧ Q) ∗ R.
+Proof.
+  intros; apply bi.persistent_and_sep_assoc; apply _.
+Qed.
+
+Lemma proj_frame:
+  forall P F ek vl,
+    proj_ret_assert (frame_ret_assert P F) ek vl ⊣⊢ F ∗ proj_ret_assert P ek vl.
+Proof.
+  intros.
+  rewrite bi.sep_comm.
+  destruct ek; simpl; rewrite ?pure_and_sep_assoc //.
+Qed.
+
+Lemma proj_conj:
+  forall P F ek vl,
+    proj_ret_assert (conj_ret_assert P F) ek vl ⊣⊢ F ∧ proj_ret_assert P ek vl.
+Proof.
+  intros.
+  rewrite bi.and_comm.
+  destruct ek; simpl; rewrite /= ?assoc //.
+Qed.
+
+Definition loop1_ret_assert (Inv: assert) (R: ret_assert) : ret_assert :=
+  {| RA_normal := Inv;
+     RA_break := RA_normal R;
+     RA_continue := Inv;
+     RA_return := RA_return R |}.
+
+Definition loop2_ret_assert (Inv: assert) (R: ret_assert) : ret_assert :=
+  {| RA_normal := Inv;
+     RA_break := RA_normal R;
+     RA_continue := False;
+     RA_return := RA_return R |}.
+
+Lemma frame_for1:
+  forall Q R F,
+   (frame_ret_assert (loop1_ret_assert Q R) F =
+    loop1_ret_assert (Q ∗ F) (frame_ret_assert R F))%stdpp.
+Proof.
+intros. reflexivity.
+Qed.
+
+Lemma frame_loop1:
+  forall Q R F,
+   (frame_ret_assert (loop2_ret_assert Q R) F ≡
+    loop2_ret_assert (Q ∗ F) (frame_ret_assert R F))%stdpp.
+Proof.
+split3; last split; try done; simpl.
+apply bi.sep_False.
+Qed.
+
+Lemma overridePost_normal:
+  forall P Q, overridePost P (normal_ret_assert Q) = normal_ret_assert P.
+Proof.
+intros; reflexivity.
+Qed.
+
+Definition bind_ret (vl: option val) (t: type) (Q: assert) : assert :=
+     match vl, t with
+     | None, Tvoid => assert_of (fun rho => Q (make_args nil nil rho))
+     | Some v, _ => ⌜tc_val t v⌝ ∧
+                               assert_of (fun rho => Q (make_args (1%positive::nil) (v::nil) rho))
+     | _, _ => False
+     end.
+
+Definition function_body_ret_assert (ret: type) (Q: assert) : ret_assert :=
+ {| RA_normal := bind_ret None ret Q;
+    RA_break := False; 
+    RA_continue := False;
+    RA_return := fun vl => bind_ret vl ret Q |}.
+
+Global Instance bind_ret_proper vl t : Proper (base.equiv ==> base.equiv) (bind_ret vl t).
+Proof.
+  intros ???; destruct vl; simpl.
+  - split => rho; monPred.unseal; rewrite /= H //.
+  - destruct t; try done.
+    split => rho; rewrite /= H //.
+Qed.
+
+Global Instance function_body_ret_assert_proper ret : Proper (base.equiv ==> base.equiv) (function_body_ret_assert ret).
+Proof.
+  intros ???; split3; last split; simpl; try done.
+  - destruct ret; try done.
+    split => rho; rewrite /= H //.
+  - intros; rewrite H //.
+Qed.
+
+Global Instance normal_ret_assert_proper : Proper (base.equiv ==> base.equiv) normal_ret_assert.
+Proof.
+  intros ???; split3; last split; simpl; try done.
+Qed.
+
+Global Instance frame_ret_assert_proper : Proper (base.equiv ==> base.equiv ==> base.equiv) frame_ret_assert.
+Proof.
+  intros ?? H ?? H'; split3; last split; simpl; intros; rewrite H'; f_equiv; apply H.
+Qed.
+
+Global Instance existential_ret_assert_proper {A} : Proper (pointwise_relation A base.equiv ==> base.equiv) existential_ret_assert.
+Proof.
+  intros ???; split3; last split; simpl; intros; do 2 f_equiv; apply H.
+Qed.
+
+End assert.
